q.sml
@@ -90,3 +90,4 @@ fun ex2fsym fsym strl th =
 
 
 
+(*TODO: q gen, qgenl*)
